Started verifying the bottom-up merge sort.

examples/miniML/hol2miniml/okasaki-examples/BottomUpMergeSortScript.sml
@@ -1,5 +1,5 @@
 open preamble
-open miscTheory ml_translatorLib;
+open miscTheory sortingTheory ml_translatorLib;
 
 val _ = new_theory "BottomUpMergeSort"
 
@@ -10,6 +10,24 @@ val _ = new_theory "BottomUpMergeSort"
 
 val _ = type_abbrev ("sortable", ``:num # 'a list list``);
 
+val sortable_inv_def = tDefine "sortable_inv" `
+(sortable_inv leq (n,[]) m = (n = 0)) ∧
+(sortable_inv leq (n,xs::xss) m =
+  if (n = 0) then
+    F
+  else if n MOD 2 = 0 then 
+    sortable_inv leq (n DIV 2,xs::xss) (m * 2)
+  else 
+    (LENGTH xs = m) ∧
+    SORTED leq xs ∧
+    sortable_inv leq (n DIV 2, xss) (m * 2))`
+(wf_rel_tac `measure (\(x,(y,z),s). y)` >>
+ rw [] >>
+ Cases_on `n = 0` >>
+ full_simp_tac (srw_ss()++ARITH_ss) []);
+
+val sortable_inv_ind = fetch "-" "sortable_inv_ind"
+
 val mrg_def = mlDefine `
 (mrg leq [] ys = ys) ∧
 (mrg leq xs [] = xs) ∧
@@ -18,6 +36,8 @@ val mrg_def = mlDefine `
     x :: mrg leq xs (y::ys)
   else
     y :: mrg leq (x::xs) ys)`;
+
+val mrg_ind = fetch "-" "mrg_ind"
 
 val empty_def = mlDefine `
 empty = (0, [])`;
@@ -36,6 +56,8 @@ add_seg leq seg segs size =
  Cases_on `size = 0` >>
  full_simp_tac (srw_ss()++ARITH_ss) []);
 
+val add_seg_ind = fetch "-" "add_seg_ind"
+
 val _ = translate add_seg_def;
 
 val add_def = mlDefine `
@@ -46,7 +68,91 @@ val mrg_all_def = mlDefine `
 (mrg_all leq xs (seg::segs) = mrg_all leq (mrg leq xs seg) segs)`;
 
 val sort_def = mlDefine `
-sort leq size segs = mrg_all leq [] segs`;
+sort leq (size, segs) = mrg_all leq [] segs`;
+
+
+
+(* Functional correctness *)
+
+val mrg_sorted = Q.prove (
+`!leq xs ys. 
+  WeakLinearOrder leq ∧ SORTED leq xs ∧ SORTED leq ys 
+  ⇒ 
+  SORTED leq (mrg leq xs ys)`,
+recInduct mrg_ind >>
+rw [SORTED_DEF,mrg_def] >|
+[cases_on `xs`, cases_on `ys`] >>
+fs [SORTED_DEF, mrg_def] >>
+every_case_tac >>
+fs [SORTED_DEF] >>
+metis_tac [WeakLinearOrder_neg]);
+
+val mrg_perm = Q.prove (
+`!leq xs ys. PERM (mrg leq xs ys) (xs++ys)`,
+recInduct mrg_ind >>
+rw [mrg_def] >>
+metis_tac [PERM_FUN_APPEND, PERM_CONS_IFF, CONS_PERM, PERM_SWAP_AT_FRONT,
+           PERM_TRANS, PERM_REFL]);
+
+val mrg_length = Q.prove (
+`!leq xs ys. LENGTH (mrg leq xs ys) = LENGTH xs + LENGTH ys`,
+recInduct mrg_ind >>
+srw_tac [ARITH_ss] [mrg_def]);
+
+val odd_div_add1 = mk_thm ([],
+``!n:num. ~EVEN n ⇒ (n DIV 2 + 1 = (n + 1) DIV 2)``);
+
+val add_seg_sub_inv = Q.prove (
+`!leq size segs n seg. 
+  WeakLinearOrder leq ∧
+  (n ≠ 0) ∧
+  sortable_inv leq (size,segs) n ∧ 
+  SORTED leq seg ∧
+  (LENGTH seg = n)
+  ⇒
+  sortable_inv leq (size+1, add_seg leq seg segs size) n`,
+recInduct sortable_inv_ind >>
+rw [] >|
+[fs [Once sortable_inv_def] >>
+     rw [Once add_seg_def] >>
+     rw [Once sortable_inv_def] >>
+     rw [Once sortable_inv_def],
+ `n ≠ 0` by fs [Once sortable_inv_def] >>
+     cases_on `n MOD 2 = 0` >>
+     fs [] >>
+     fs [Once sortable_inv_def] >>
+     rw [Once add_seg_def] >>
+     rw [Once sortable_inv_def] >|
+     [fs [arithmeticTheory.MOD_2] >>
+          every_case_tac >>
+          fs [arithmeticTheory.EVEN_ADD],
+      `0 < 2:num` by rw [] >>
+          `(n+1) DIV 2 = n DIV 2 + 1 DIV 2`  
+                     by metis_tac [arithmeticTheory.ADD_DIV_RWT] >>
+          fs [],
+      `LENGTH seg + LENGTH xs = LENGTH seg * 2`
+                    by decide_tac >>
+          `sortable_inv leq (n DIV 2 +  1, 
+                             add_seg leq (mrg leq seg xs) xss (n DIV 2)) 
+                        (LENGTH seg * 2)`
+                    by metis_tac [mrg_sorted, mrg_length] >>
+          cases_on `add_seg leq (mrg leq seg xs) xss (n DIV 2)` >>
+          fs [] >-
+          fs [Once sortable_inv_def] >>
+          rw [Once sortable_inv_def] >>
+          fs [arithmeticTheory.MOD_2] >>
+          every_case_tac >>
+          fs [arithmeticTheory.EVEN_ADD] >>
+          metis_tac [odd_div_add1]]]);
+
+val add_correct = Q.store_thm ("add_correct",
+`!leq x size segs. 
+  WeakLinearOrder leq ∧ sortable_inv leq (size,segs) 1
+  ⇒ 
+  sortable_inv leq (add leq x (size,segs)) 1`,
+rw [add_def] >>
+match_mp_tac add_seg_sub_inv >>
+rw [SORTED_DEF]);
 
 
 (* translation *)
